removed ComputableTime from L

theories/L/Functions/EqBool.v
@@ -21,25 +21,9 @@ Proof.
   intros ? ?. eapply iff_reflect. rewrite eqb_true_iff. reflexivity.
 Qed.
 
-Lemma dec_reflect_remove {P Y} (d:dec P) b (H:reflect P b) (y y' : Y):
-  (if d then y else y') = (if b then y else y').
-Proof.
-  destruct H,d;easy.
-Qed.
-
-Lemma eqDec_remove {X Y eqb} {H:eqbClass (X:=X) eqb} x x' (d:dec (x=x')) (a b : Y):
-  (if d then a else b) = (if eqb x x' then a else b).
-Proof.
-  apply dec_reflect_remove. eapply eqb_spec.
-Qed.
-
-Class eqbCompT X {R:encodable X} eqb {H:eqbClass (X:=X) eqb} :=
-  { c__eqbComp :nat;
-    eqbTime x y:= min x y* c__eqbComp;
-    comp_eqb : computableTime' eqb (fun x _ =>(5,fun y _ => (eqbTime (size (enc x)) (size (enc y)),tt)))
-  }.
+Class eqbCompT X {R:registered X} eqb {H:eqbClass (X:=X) eqb} :=
+  { comp_eqb : computable eqb }.
 Arguments eqbCompT _ {_ _ _}.
-Arguments c__eqbComp _ {_ _ _ _}.
 
 #[export] Hint Mode eqbCompT + - - -: typeclass_instances.
 
@@ -47,35 +31,7 @@ Arguments c__eqbComp _ {_ _ _ _}.
 Existing Instance comp_eqb.
 
 #[global]
-Instance eqbComp_bool : eqbCompT bool.
+Instance term_eqb_bool : computable Bool.eqb.
 Proof.
-  evar (c:nat). exists c. unfold Bool.eqb.
-  unfold enc;cbn.
   extract.
-  solverec.
-  [c]:exact 3.
-  all:unfold c;try lia.
 Qed.
-
-Lemma eqbTime_le_l X {R : encodable X} (eqb : X -> X -> bool) {H : eqbClass eqb}
-      {H' : eqbCompT X} x n':
-  eqbTime (X:=X) x n' <= x * c__eqbComp X.
-Proof.
-  unfold eqbTime. rewrite Nat.le_min_l. easy.
-Qed.
-
-Lemma eqbTime_le_r X (R : encodable X) (eqb : X -> X -> bool) (H : eqbClass eqb)
-      (eqbCompT : eqbCompT X) x n':
-  eqbTime (X:=X) n' x <= x * c__eqbComp X.
-Proof.
-  unfold eqbTime. rewrite Nat.le_min_r. easy.
-Qed.
-
-(*
-Lemma eqbTime_upToC X {R:encodable X} eqb {H:eqbClass (X:=X) eqb} {_:eqbCompT X}:
-  eqbTime (X:=X) <=c (fun (x y:nat) => min x y).
-Proof.
-  unfold eqbTime. hnf.
-  exists (c__eqbComp X). unfold leHO;repeat intro; cbn;nia.
-Qed.
-*)
