theories/L/Datatypes/LNat.v
@@ -1,210 +1,97 @@
-From Undecidability.L Require Export Util.L_facts.
+
 From Undecidability.L.Tactics Require Export LTactics GenEncode.
-Require Import Undecidability.Shared.Libs.PSL.Numbers.
 
 Require Import Nat.
-From Undecidability.L Require Import Datatypes.LBool Functions.EqBool Datatypes.LProd. 
-Import GenEncode. Import Nat.
+From Undecidability.L Require Import Datatypes.LBool Functions.EqBool Datatypes.LProd.
+Import GenEncode.
 (* ** Encoding of natural numbers *)
 
-MetaCoq Run (tmGenEncodeInj "nat_enc" nat).
+MetaCoq Run (tmGenEncode "nat_enc" nat).
 #[export] Hint Resolve nat_enc_correct : Lrewrite.
 
 #[global]
-Instance termT_S : computableTime' S (fun _ _ => (1,tt)).
+Instance termT_S : computable S.
 Proof.
   extract constructor.
-  solverec.
 Qed.
 
 #[global]
-Instance termT_pred : computableTime' pred (fun _ _ => (5,tt)).
+Instance termT_pred : computable pred.
 Proof.
   extract.
-  solverec.
 Qed.
 
-Definition c__add := 11. 
-Definition c__add1 := 5.
-Definition add_time x := (x + 1) * c__add.
 #[global]
-Instance termT_plus' : computableTime' add (fun x xT => (c__add1,(fun y yT => (add_time x,tt)))).
+Instance termT_plus' : computable add.
 Proof.
   extract.
-  fold add. solverec. 
-  all: unfold add_time, c__add1, c__add; solverec. 
 Qed.
 
-Definition c__mult1 := 5.
-Definition c__mult := c__add + c__add1 + 10.
-Definition mult_time x y := x * y * c__mult + c__mult * (x+ 1) .
 #[global]
-Instance termT_mult : computableTime' mult (fun x xT => (c__mult1,(fun y yT => (mult_time x y,tt)))).
-Proof.
-  extract. solverec. 
-  all: unfold mult_time, c__mult1, c__mult, add_time, c__add1, c__add; solverec. 
-Qed.
-
-Definition c__sub1 := 5.
-Definition c__sub := 14. 
-Definition sub_time x y := (min x y + 1) * c__sub.
-#[global]
-Instance term_sub : computableTime' Nat.sub (fun n _ => (c__sub1,fun m _ => (sub_time n m ,tt)) ).
-Proof.
-  extract. solverec.
-  all: unfold sub_time, c__sub1, c__sub; solverec. 
-Qed.
-
-Definition c__leb := 14.
-Definition c__leb2 := 5. 
-Definition leb_time (x y : nat) := c__leb * (1 + min x y).
-#[global]
-Instance termT_leb : computableTime' leb (fun x xT => (c__leb2,(fun y yT => (leb_time x y,tt)))).
+Instance termT_mult : computable mult.
 Proof.
   extract.
-  solverec. all: unfold leb_time, c__leb, c__leb2; solverec. 
 Qed.
 
-Definition c__ltb := c__leb2 + 4.
-Definition ltb_time (a b : nat) := leb_time (S a) b + c__ltb. 
 #[global]
-Instance term_ltb : computableTime' Nat.ltb (fun a _ => (1, fun b _ => (ltb_time a b, tt))). 
-Proof. 
-  extract. recRel_prettify2. 
-  - lia. 
-  - unfold ltb_time, c__ltb. solverec. 
+Instance term_sub : computable Nat.sub.
+Proof.
+  extract.
+Qed.
+
+#[global]
+Instance termT_leb : computable leb.
+Proof.
+  extract.
+Qed.
+
+#[global]
+Instance term_ltb : computable Nat.ltb.
+Proof.
+  extract.
 Qed.
 
 #[global]
 Instance eqbNat_inst : eqbClass Nat.eqb.
 Proof.
-  exact Nat.eqb_spec. 
+  exact Nat.eqb_spec.
 Qed.
 
 #[global]
-Instance eqbComp_nat : eqbCompT nat.
+Instance term_eqb_nat : computable Nat.eqb.
 Proof.
-  evar (c:nat). exists c. unfold Nat.eqb.
-  unfold enc;cbn.
   extract.
-  solverec.
-  [c]:exact 5.
-  all:unfold c;try lia.
 Qed.
-(*Qed.*)
 
-Definition c__min1 := 5.
-Definition c__min2 := 15. 
-Definition min_time x y := (min x y + 1) * c__min2. 
 #[global]
-Instance termT_nat_min : computableTime' Nat.min (fun x _ => (c__min1, fun y _ => (min_time x y, tt))).
-Proof. 
-  extract. solverec. 
-  all: unfold min_time, c__min1, c__min2; solverec. 
+Instance termT_nat_min : computable Nat.min.
+Proof.
+  extract.
+Qed.
+
+#[global]
+Instance termT_nat_max : computable Nat.max.
+Proof.
+  extract.
 Qed. 
 
-Definition c__max1 := 5.
-Definition c__max2 := 15. 
-Definition max_time x y := (min x y + 1) * c__max2. 
-#[global]
-Instance termT_nat_max : computableTime' Nat.max (fun x _ => (c__max1, fun y _ => (max_time x y, tt))).
-Proof. 
-  extract. solverec. 
-  all: unfold max_time, c__max1, c__max2; solverec. 
-Qed. 
-
-Definition c__pow1 := 5.
-Definition c__pow2 := 10 + c__mult1.
-Fixpoint pow_time x n := match n with 
-  | 0 => c__pow2 
-  | S n => pow_time x n + mult_time x (x ^n) + c__pow2
-end.
 #[global]
 Instance termT_pow:
-  computableTime' Init.Nat.pow   (fun (x : nat) _ => (c__pow1,fun (n : nat) _ => (pow_time x n, tt))).
+  computable Init.Nat.pow.
 Proof.
-  extract. fold Nat.pow. solverec. 
-  all: unfold pow_time, c__pow1, c__pow2; solverec. 
+  extract.
 Qed.
 
-
-Definition c__divmod := 20.
-Definition divmod_time (x: nat) := c__divmod * (1+x).
 #[global]
-Instance termT_divmod : 
-  computableTime' divmod (fun (x : nat) _ => (5, fun (y : nat) _ => (5, fun (q : nat) _ => (1, fun (u : nat) _ => (divmod_time x, tt))))). 
-Proof. 
-  extract. solverec. all: unfold divmod_time, c__divmod; solverec. 
+Instance termT_divmod :
+  computable divmod.
+Proof.
+  extract.
 Qed. 
 
-Definition c__modulo := 21 + c__sub1. 
-Definition modulo_time (x :nat) (y : nat) := divmod_time x + c__sub * y + c__modulo.
 #[global]
-Instance termT_modulo : 
-  computableTime' Init.Nat.modulo (fun x _ => (1, fun y _ => (modulo_time x y, tt))). 
-Proof. 
-  extract. solverec. 
-  - unfold modulo_time, c__modulo; solverec. 
-  - unfold sub_time. rewrite Nat.le_min_l. unfold modulo_time, c__modulo. solverec. 
-Qed. 
-
-(* now some more encoding-related properties:*)
-
-Fixpoint nat_unenc (s : term) :=
-  match s with
-  | lam (lam #1) => Some 0
-  | lam (lam (app #0 s)) => match nat_unenc s with Some n => Some (S n) | x=>x end
-  | _ => None
-  end.
-
-Lemma unenc_correct m : (nat_unenc (nat_enc m)) = Some m.
+Instance termT_modulo :
+  computable Init.Nat.modulo.
 Proof.
-  induction m; simpl; now try rewrite IHm.
+  extract.
 Qed.
-
-Lemma unenc_correct2 t n : nat_unenc t = Some n -> nat_enc n = t.
-Proof with try solve [Coq.Init.Tactics.easy].
-  revert n. eapply (size_induction (f := size) (p := (fun t => forall n, nat_unenc t = Some n -> nat_enc n = t))). clear t. intros t IHt n H.
-  destruct t as [ | | t]. easy. easy.
-  destruct t as [ | | t]. easy. easy.
-  destruct t. 3:easy.
-  -destruct n0. easy. destruct n0. 2:easy. inv H. easy.
-  -destruct t1. 2-3:easy. destruct n0. 2:easy. simpl in H. destruct (nat_unenc t2) eqn:A.
-   +apply IHt in A;simpl;try lia. destruct n. inv H. simpl. congruence.
-   +congruence.
-Qed.
-
-Lemma dec_enc t : dec (exists n, t = nat_enc n).
-Proof.
-  destruct (nat_unenc t) eqn:H.
-  - left. exists n. now eapply unenc_correct2 in H.
-  - right. intros [n A]. rewrite A in H. rewrite unenc_correct in H. inv H.
-Qed.
-
-Definition c__natsizeO := 4.
-Definition c__natsizeS := 4.
-Lemma size_nat_enc (n:nat) :
-  size (enc n) = n * c__natsizeS + c__natsizeO.
-Proof.
-  unfold c__natsizeS, c__natsizeO. 
-  induction n;cbv [enc encodable_nat_enc] in *. all:cbn [size nat_enc] in *. all:solverec.
-Qed.
-
-Lemma size_nat_enc_r (n:nat) :
-  n <= size (enc n).
-Proof.
-    induction n;cbv [enc encodable_nat_enc] in *. all:cbn [size nat_enc] in *. all:solverec.
-Qed.
-
-
-(* This is an example for an function in which the run-time of the fix itself is not constant (in add, the fix on the first argument always returns an function in ~5 steps)*)
-(* Instance termT_testId : computableTime' (fix f x := *)
-(*                                             match x with *)
-(*                                               0 => 0 *)
-(*                                             | S x => S (f x) *)
-(*                                             end). *)
-(* Proof. *)
-(*   extract. *)
-(*   eexists (fun x xT => (x*9+7,tt)). *)
-(*   abstract (repeat (cbn;intros;intuition;try destruct _;try ring_simplify)). *)
-(* Qed. *)
