theories/L/Datatypes/LOptions.v
@@ -1,46 +1,21 @@
 From Undecidability.L Require Import Tactics.LTactics Datatypes.LBool Tactics.GenEncode.
 From Undecidability.L Require Import Functions.EqBool.
-Import L_Notations.
 
 (* ** Encoding of option type *)
 Section Fix_X.
   Variable X:Type.
-  Context {intX : encodable X}.
-
+  Context {intX : registered X}.
 
   MetaCoq Run (tmGenEncode "option_enc" (option X)).
   Hint Resolve option_enc_correct : Lrewrite.
 
-  Global Instance encInj_option_enc {H : encInj intX} : encInj (encodable_option_enc).
-  Proof. register_inj. Qed. 
-  
   (* now we must register the non-constant constructors*)
 
-  Global Instance term_Some : computableTime' (@Some X) (fun _ _ => (1,tt)).
+  Global Instance term_Some : computable (@Some X).
   Proof.
     extract constructor.
-    solverec.
   Defined. (*because next lemma*)
 
-  Lemma oenc_correct_some (s: option X) (v : term) : lambda v -> enc s == ext (@Some X) v -> exists s', s = Some s' /\ v = enc s'.
-  Proof.
-    intros lam_v H. unfold ext in H;cbn in H. unfold extT in H; cbn in H. redStep in H.
-    apply unique_normal_forms in H;[|Lproc..]. destruct s;simpl in H.
-    -injection H;eauto.
-    -discriminate H.
-  Qed.
-       
-
-
-   (*
-   Lemma none_equiv_some v : proc v -> ~ none == some v.
-   Proof.
-     intros eq. rewrite some_correct. Lrewrite. apply unique_normal_forms in eq;[discriminate|Lproc..].
-     intros H. assert (converges (some v)) by (eexists; split;[rewrite <- H; cbv; now unfold none| auto]). destruct (app_converges H0) as [_ ?]. destruct H1 as [u [H1 lu]]. rewrite H1 in H.
-     symmetry in H. eapply eqTrans with (s := (lam (lam (#1 u)))) in H.
-     eapply eq_lam in H. inv H. symmetry. unfold some. clear H. old_Lsimpl.
-   Qed.
-    *)
 End Fix_X.
 
 #[export] Hint Resolve option_enc_correct : Lrewrite.
@@ -68,14 +43,11 @@ End option_eqb.
 Section int.
 
   Variable X:Type.
-  Context {HX : encodable X}.
+  Context {HX : registered X}.
 
-  Global Instance term_option_eqb : computableTime' (@option_eqb X)
-                                                    (fun eqb eqbT => (1, fun a _ => (1,fun b _ => (match a,b with
-                                                                                            Some a, Some b => callTime2 eqbT a b + 10
-                                                                                          | _,_ => 8 end,tt)))). cbn.
+  Global Instance term_option_eqb : computable (@option_eqb X).
   Proof.
-    extract. solverec.
+    extract.
   Qed.
 
   Global Instance eqbOption f `{eqbClass (X:=X) f}:
@@ -83,34 +55,13 @@ Section int.
   Proof.
     intros ? ?. eapply option_eqb_spec. all:eauto using eqb_spec.
   Qed.
-
-  Global Instance eqbComp_Option `{H:eqbCompT X (R:=HX)}:
-    eqbCompT (option X).
-  Proof.
-    evar (c:nat). exists c. unfold option_eqb. 
-    unfold enc;cbn.
-    change (eqb0) with (eqb (X:=X)).
-    extract. unfold eqb,eqbTime.
-    recRel_prettify2. easy.
-    [c]:exact (c__eqbComp X + 6).
-    all:set (f:=enc (X:=option X)); unfold enc in f;subst f;cbn [size].
-    all:unfold c. all:nia. 
-  Qed.
-
 End int.
 
 Definition isSome {T} (u : option T) := match u with Some _ => true | _ => false end.
 
 #[global]
-Instance term_isSome {T} `{encodable T} : computable (@isSome T).
+Instance term_isSome {T} `{registered T} : computable (@isSome T).
 Proof.
   extract.
 Qed.
 
-
-Lemma size_option X `{encodable X} (l:option X):
-  size (enc l) = match l with Some x => size (enc x) + 5 | _ => 3 end.
-Proof.
-  unfold enc at 1.
-  destruct l. all:cbn; nia.
-Qed.
