theories/L/Datatypes/LUnit.v
@@ -1,10 +1,6 @@
-From Undecidability.L Require Export Util.L_facts.
-From Undecidability.L.Tactics Require Import LTactics GenEncode.
+From Undecidability.L.Tactics Require Import GenEncode.
 (* * Encodings and extracted basic functions *)
 (* ** Encoding of unit *)
 
-MetaCoq Run (tmGenEncodeInj "unit_enc" unit).
+MetaCoq Run (tmGenEncode "unit_enc" unit).
 #[export] Hint Resolve unit_enc_correct : Lrewrite.
-
-Lemma size_unit_enc : size(enc tt) = 2. 
-Proof. reflexivity. Qed. 
