theories/L/Datatypes/List/List_eqb.v
@@ -5,7 +5,7 @@ From Undecidability.L.Datatypes Require Export List.List_enc LBool LOptions LNat
 
 Section Fix_X.
   Variable (X:Type).
-  Context {intX : encodable X}.
+  Context {intX : registered X}.
 
   Fixpoint inb eqb (x:X) (A: list X) :=
     match A with
@@ -28,20 +28,10 @@ Section Fix_X.
       *constructor. tauto.
   Qed.
 
-  Global Instance term_inb: computableTime' inb (fun eq eqT => (5,fun x _ => (1,fun l _ =>
-                                        (fold_right (fun x' res => callTime2 eqT x' x
-                                                                + res + 17) 4 l ,tt)))).
-  Proof.
-    extract.
-    solverec. 
-  Defined. (*because other extract*)
-
   Global Instance term_inb_notime: computable inb.
   Proof.
     extract.
   Defined. (*because other extract*)
-
-
 
 End Fix_X.
 
@@ -69,43 +59,11 @@ End list_eqb.
 Section int.
 
   Context {X : Type}.
-  Context {HX : encodable X}.
+  Context {HX : registered X}.
 
-  Fixpoint list_eqbTime (eqbT: timeComplexity (X -> X -> bool)) (A B:list X) :=
-    match A,B with
-      a::A,b::B => callTime2 eqbT a b + 22 + list_eqbTime eqbT A B
-    | _,_ => 9
-    end.
-
-  Global Instance term_list_eqb : computableTime' (list_eqb (X:=X))
-                                                  (fun _ eqbT => (1,(fun A _ => (5,fun B _ => (list_eqbTime eqbT A B,tt))))).
+  Global Instance term_list_eqb : computable (list_eqb (X:=X)).
   Proof.
-    extract.
-    solverec.                                                                                             
-  Qed.
-
-  Definition list_eqbTime_leq (eqbT: timeComplexity (X -> X -> bool)) (A B:list X) k:
-    (forall a b, callTime2 eqbT a b <= k)
-    -> list_eqbTime eqbT A B <= length A * (k+22) + 9.
-  Proof.
-    intros H'. induction A in B|-*.
-    -cbn. lia.
-    -destruct B.
-    {cbn. intuition. }
-    cbn - [callTime2]. setoid_rewrite IHA.
-    rewrite H'. ring_simplify. intuition.
-  Qed.
-
-
-  Lemma list_eqbTime_bound_r (eqbT : timeComplexity (X -> X -> bool)) (A B : list X) f:
-    (forall (x y:X), callTime2 eqbT x y <= f y) ->
-    list_eqbTime eqbT A B <= sumn (map f B) + 9 + length B * 22.
-  Proof.
-    intros H.
-    induction A in B|-*;unfold list_eqbTime;fold list_eqbTime. now Lia.lia.
-    destruct B.
-    -cbn. Lia.lia.
-    -rewrite H,IHA. cbn [length map sumn]. Lia.lia.
+    extract.                                                                                        
   Qed.
 
   Global Instance eqbList f `{eqbClass (X:=X) f}:
@@ -114,14 +72,5 @@ Section int.
     intros ? ?. eapply list_eqb_spec. all:eauto using eqb_spec.
   Qed.
   Import EqBool.
-  Global Instance eqbComp_List `{eqbCompT X (R:=HX)}:
-    eqbCompT (list X).
-  Proof.
-    evar (c:nat). exists c. unfold list_eqb.
-    extract. unfold eqb,eqbTime. cbn - ["+"].
-    [c]:exact (c__eqbComp X + 6).
-    all:unfold c. set (c__eqbComp X). 
-    solverec. all: set (f:=enc (X:=list X)); unfold enc in f;subst f;cbn [size encodable_list_enc].
-    all:try nia. 
-  Qed.
+  
 End int.
