theories/L/Datatypes/List/List_fold.v
@@ -5,63 +5,32 @@ Section forallb.
   Variable (X : Type).
   Context (H : encodable X).
 
-  Definition c__forallb := 15. 
-  Definition forallb_time (fT : X -> nat) (l : list X) := sumn (map (fun elm => fT elm + c__forallb) l) + c__forallb. 
-
-  Global Instance term_forallb : computableTime' (@forallb X) (fun f fT => (1, fun l _ => (forallb_time (callTime fT) l, tt))). 
+  Global Instance term_forallb : computable (@forallb X). 
   Proof.
     extract.
-    solverec. 
-    all: unfold forallb_time, c__forallb; solverec. 
   Qed. 
 
-  Lemma forallb_time_eq f (l:list X):
-    forallb_time f l = sumn (map f l) + length l * c__forallb + c__forallb.
-  Proof.
-    induction l as [ | x l IH];cbn -[c__forallb]. lia. unfold forallb_time in IH. nia.
-  Qed.
-
-  Lemma forallb_time_const c (l:list X):
-    forallb_time (fun _ =>  c) l = length l * (c+c__forallb) + c__forallb.
-  Proof.
-    induction l as [ | x l IH];cbn -[c__forallb]. lia. unfold forallb_time in IH; nia.
-  Qed.
 End forallb.
 
-
-  Section foldl_time.
+Section foldl_time.
   Context {X Y : Type}.
   Context {H : encodable X}.
   Context {F : encodable Y}.
 
-  Definition c__fold_left := 15. 
-  Definition c__fold_left2 := 5.
-  Fixpoint fold_left_time (f : X -> Y -> X) (t__f : X -> Y -> nat) (l : list Y) (acc : X) :=
-  (match l with
-      | [] =>c__fold_left 
-      | (l :: ls) => t__f acc l + c__fold_left + fold_left_time f t__f ls (f acc l)
-      end ).
-
   Global Instance term_fold_left :
-    computableTime' (@fold_left X Y) (fun f fT => (c__fold_left2, fun l _ => (c__fold_left2, fun acc _ => (fold_left_time f (callTime2 fT) l acc, tt)))). 
+    computable (@fold_left X Y). 
   Proof.
-    extract. 
-    solverec. all: unfold c__fold_left, c__fold_left2; solverec. 
+    extract.
   Qed. 
 End foldl_time.
 
-  Section foldr_time.
+Section foldr_time.
   Context {X Y: Type}.
   Context {H:encodable X}.
   Context {H0: encodable Y}.
 
-  Definition c__fold_right := 15.
-  Fixpoint fold_right_time (f : Y -> X -> X) (tf : Y -> X -> nat) (l : list Y) (acc : X) :=
-      match l with [] => c__fold_right
-              | l::ls => tf l (fold_right f acc ls) + c__fold_right + fold_right_time f tf ls acc
-      end. 
-  Global Instance term_fold_right : computableTime' (@fold_right X Y) (fun f fT => (1, fun acc _ => (1, fun l _ => (fold_right_time f (callTime2 fT) l acc + c__fold_right, tt)))).
+  Global Instance term_fold_right : computable (@fold_right X Y).
   Proof.
-    extract. solverec. all: unfold fold_right, c__fold_right; solverec.  
+    extract.
   Qed. 
 End foldr_time.
