theories/L/Functions/FinTypeLookup.v
@@ -1,11 +1,11 @@
 From Undecidability.L.Tactics Require Import LTactics.
-From Undecidability.L.Datatypes Require Import LFinType LBool LProd Lists.
+From Undecidability.L.Datatypes Require Import LFinType LBool LProd.
 From Undecidability.L.Functions Require Import EqBool.
+From Undecidability.L.Datatypes.List Require Import List_enc.
 
 Section Lookup.
   Variable X Y : Type.
-  Context {eqbX : X -> X -> bool}.
-  Context `{eqbClass X eqbX}.
+  Context `{HX : eqbCompT X}.
 
   Fixpoint lookup (x:X) (A:list (X*Y)) d: Y :=
     match A with
@@ -14,27 +14,10 @@ Section Lookup.
       if eqb x key then Lproc else lookup x A d
     end.
 
-  Context `{encodable X} `{@eqbCompT X _ eqbX _}.
-
-  Definition lookupTime (x:nat) (l:list (X*Y)):=
-    fold_right (fun '(a,b) res => eqbTime (X:=X) x (size (enc (a:X))) + res +24) 4 l.
-
-  Global Instance term_lookup `{encodable Y}:
-    computableTime' (lookup) (fun x _ => (5, fun l _ => (1, fun d _ => (lookupTime (size (enc x)) l,tt)))).
-  Proof.
-  unfold lookup. unfold eqb.
-  extract. unfold lookupTime. solverec.
-  Qed.
-
-  Lemma lookupTime_leq x (l:list (X*Y)):
-    lookupTime x l <= length l * (x* c__eqbComp X + 24) + 4.
-  Proof.
-    induction l as [ | [a b] l].
-    -cbn. lia.
-    -unfold lookupTime. cbn [fold_right]. fold (lookupTime x l).
-     rewrite eqbTime_le_l.
-     setoid_rewrite IHl. cbn [length].
-     ring_simplify. unfold eqb. lia.
+  Global Instance term_lookup `{registered Y} :
+    computable (lookup).
+  Proof using HX.
+    extract.
   Qed.
 
 End Lookup.
@@ -47,7 +30,6 @@ Section funTable.
 
   Definition funTable :=
     map (fun x => (x,f x)) (elem X).
-
 
   Variable (eqbX : X -> X -> bool).
   Context `{eqbClass X eqbX}.
@@ -65,48 +47,5 @@ Section funTable.
      +destruct Hel. 1:congruence.
       eauto.
   Qed.
-  
+
 End funTable.
-
-Lemma lookup_sound' (A: Type) (B: Type) eqbA `{eqbClass (X:=A) eqbA} (L : list (prod A B)) a b def :
-  (forall a' b1 b2, (a',b1) el L -> (a',b2) el L -> b1=b2) -> ( (a,b) el L \/ ((forall b', ~ (a,b') el L) /\ b = def) ) -> lookup a L def = b.
-Proof.
-  intros H1 H2.
-  induction L as [ |[a' b'] L]. now intuition.
-  cbn.
-  destruct (eqb_spec a a').
-  -subst a. destruct H2.
-   2:now exfalso.
-   eapply H1. all:easy.
-  -apply IHL. all:intros.
-   +eapply H1. all:eauto.
-   +destruct H2 as [[]|]. all:easy.
-Qed.
-
-Lemma lookup_sound (A: Type) (B: Type) eqbA `{eqbClass (X:=A) eqbA} (L : list (A * B)) a b def : 
-  (forall a' b1 b2, (a', b1) el L -> (a', b2) el L -> b1 = b2) -> (a, b) el L -> lookup a L def = b.
-Proof. 
-  intros H1 H2. induction L; cbn; [ destruct H2 | ]. 
-  destruct a0 as [a0 b0]. specialize (H a a0) as Heqb. apply reflect_iff in Heqb.
-  unfold EqBool.eqb. 
-  destruct eqbA. 
-  - specialize (proj2 Heqb eq_refl) as ->.
-    destruct H2 as [H2 | H2]; [easy | ].
-    apply (H1 a0); easy.
-  - assert (not (a = a0)). { intros ->. easy. }
-    destruct H2 as [H2 | H2]; [ congruence | ].
-    apply IHL in H2; [easy | intros; now eapply H1]. 
-Qed. 
-
-Lemma lookup_complete (A: Type) (B: Type) eqbA `{eqbClass (X:=A) eqbA} (L : list (prod A B)) a def :
-  {(a,lookup a L def) el L } + {~(exists b, (a,b) el L) /\ lookup a L def  = def}.
-Proof.
-  induction L as [ |[a' b'] L].
-  -cbn. right. firstorder.
-  -cbn.  destruct (eqb_spec a a').
-   1:{ do 2 left. congruence. }
-   destruct IHL as [|[? eq]];[left|right].
-   +eauto.
-   +split. 2:easy.
-    now intros (?&[]). 
-Qed.
