theories/L/Prelim/MoreList.v
@@ -1,29 +1,4 @@
 Require Import Undecidability.Shared.Libs.PSL.Base Lia.
-Require Import Arith.
-(* Nats smaller than n *)
-
-Fixpoint natsLess n : list nat :=
-  match n with
-    0 => []
-  | S n => n :: natsLess n
-  end.
-
-Lemma natsLess_in_iff n m:
-  n el natsLess m <-> n < m.
-Proof.
-  induction m in n|-*;cbn. lia.
-  split.
-  -intuition. destruct n; intuition lia. apply IHm in H0. lia.
-  -intros. decide (m=n). intuition lia. right. apply IHm. lia.
-Qed.
-
-
-Lemma natsLess_S n :
-  natsLess (S n) = map S (natsLess n)++[0].
-Proof.
-  induction n;cbn in *;congruence.
-Qed.
-
 
 (* Sum *)
 
@@ -55,20 +30,6 @@ Proof.
   cbn in *. specialize (IHA (a::B)). autorewrite with list in *. cbn in *. lia.
 Qed.
 
-Lemma sumn_map_natsLess f n :
-  sumn (map f (natsLess n)) = sumn (map (fun i => f (n - (1 + i))) (natsLess n)).
-Proof.
-  rewrite sumn_rev. f_equal.
-  rewrite <- map_rev.
-  rewrite <- map_map with (g:=f) (f:= fun i => (n - (1+i))).
-  f_equal.
-  induction n;intros;autorewrite with list in *. reflexivity.
-  rewrite natsLess_S at 2. cbn. rewrite map_app. cbn.
-  rewrite map_map. cbn in IHn.
-  rewrite IHn. rewrite <- minus_n_O. reflexivity.
-Qed.
-
-
 Lemma sumn_map_add X f g (l:list X) :
   sumn (map (fun x => f x + g x) l) = sumn (map f l) + sumn (map g l).
 Proof.
@@ -96,34 +57,8 @@ Proof.
   induction xs;cbn. easy. etransitivity. apply sumn_app. nia.
 Qed.
 
-
 Lemma sumn_repeat c n: sumn (repeat c n) = c * n.
 Proof.
   induction n;cbn. all:nia.
 Qed.
 
-Definition maxl := fold_right max 0.
-Lemma maxl_leq n l: n el l -> n <= maxl l.
-Proof.
-  induction l;cbn.
-  -easy.
-  -intros [->|]. all:apply Nat.max_case_strong;try intuition Lia.lia.
-Qed.
-
-Lemma maxl_leq_l c l :
-  (forall n, n el l -> n <= c) -> maxl l <= c.
-Proof.
-  induction l;cbn. Lia.lia. 
-  intros H. eapply Nat.max_lub_iff;split. all:eauto.  
-Qed.
-
-Lemma maxl_app l l': maxl (l++l') = max (maxl l) (maxl l').
-Proof.
-  induction l;cbn;Lia.lia.
-Qed.
-
-Lemma maxl_rev l: maxl (rev l) = maxl l.
-Proof.
-  unfold maxl. rewrite fold_left_rev_right. rewrite fold_symmetric. 2,3:now intros;Lia.lia.
-  induction l;cbn;try Lia.lia.
-Qed.
