theories/L/Reductions/HaltL_to_HaltLclosed.v
@@ -1,6 +1,6 @@
 
 Require Import Undecidability.Synthetic.Definitions.
-From Undecidability.L Require Import L Functions.Eval.
+From Undecidability.L Require Import L Computability.Seval Functions.Eval Computability.MuRec.
 Import L_Notations.
 
 (* Halting problem for call-by-value lambda-calculus *)
@@ -11,8 +11,8 @@ Proof.
   unshelve eexists.
   - intros s. exists (Eval (enc s)). unfold Eval. Lproc. 
   - cbn. intros s. unfold HaltL. split; intros (t & Ht).
-    + eapply Seval.converges_eval. edestruct Eval_converges. eapply H.
+    + eapply converges_eval. edestruct Eval_converges. eapply H.
       eapply eval_iff in Ht. eauto.
-    + setoid_rewrite eval_iff. cbn in Ht. eapply Seval.converges_eval.
-      eapply Eval_converges. eapply Seval.eval_converges. eauto.
+    + setoid_rewrite eval_iff. cbn in Ht. eapply converges_eval.
+      eapply Eval_converges. eapply eval_converges. eauto.
 Qed.
