theories/L/TM/TMEncoding.v
@@ -1,5 +1,7 @@
 From Undecidability.L.Tactics Require Import LTactics GenEncode.
-From Undecidability.L.Datatypes Require Import LNat Lists LProd LFinType LVector.
+From Undecidability.L.Datatypes Require Import LNat LProd LFinType LVector.
+From Undecidability.L.Datatypes.List Require Import List_basics List_eqb List_fold List_enc.
+
 From Undecidability.L Require Import Functions.EqBool.
 
 From Undecidability.TM.Util Require Import VectorPrelim TM_facts.
@@ -13,7 +15,7 @@ Import L_Notations.
 (* ** Extraction of Turing Machine interpreter  *)
 
 Import GenEncode.
-MetaCoq Run (tmGenEncodeInj "move_enc" move).
+MetaCoq Run (tmGenEncode "move_enc" move).
 #[export] Hint Resolve move_enc_correct : Lrewrite.
 
 Import TM.
@@ -42,45 +44,10 @@ Proof.
   intros ? ?. eapply move_eqb_spec.
 Qed.
 
-
-#[global]
-Instance eqbComp_bool : eqbCompT move.
-Proof.
-  evar (c:nat). exists c. unfold move_eqb.
-  unfold enc;cbn.
-  extract.
-  solverec.
-  [c]:exact 3.
-  all:unfold c;try lia.
-Qed.
-
-(*
-Definition move_decode (s : term) : option (move) :=
-  match s with
-  | lam (lam (lam n)) =>
-    match n with
-      2 => Some TM.L 
-    | 1 => Some TM.R
-    | 0 => Some TM.N
-    | _ => None
-    end
-  | _ => None
-  end.
-
-Instance decode_move: decodable move.
-Proof.
-  exists move_decode.
-  all:unfold enc at 1. all:cbn.
-  -destruct x;reflexivity.
-  -destruct t eqn:eq. all:cbn.
-   all:repeat let eq := fresh in destruct _ eqn:eq. all:try congruence.
-   all:intros ? [= <-]. all:reflexivity.
-Defined. (* because instance *) *)
-
 (* *** Encoding Tapes *)
 Section reg_tapes.
   Variable sig : Type.
-  Context `{reg_sig : encodable sig}.
+  Context `{reg_sig : registered sig}.
 
   
   Implicit Type (t : TM.tape sig).
@@ -88,25 +55,21 @@ Section reg_tapes.
   MetaCoq Run (tmGenEncode "tape_enc" (TM.tape sig)).
   Hint Resolve tape_enc_correct : Lrewrite.
 
-  Global Instance encInj_tape_enc {H : encInj reg_sig} : encInj (encodable_tape_enc).
-  Proof. register_inj. Qed. 
-
   (*Internalize constructors **)
 
-  Global Instance term_leftof : computableTime' (@leftof sig) (fun _ _ => (1, fun _ _ => (1,tt))).
+  Global Instance term_leftof : computable (@leftof sig).
   Proof.
     extract constructor.
-    solverec.
   Qed.
 
-  Global Instance term_rightof : computableTime' (@rightof sig) (fun _ _ => (1, fun _ _ => (1,tt))).
+  Global Instance term_rightof : computable (@rightof sig).
   Proof.
-    extract constructor. solverec.
+    extract constructor.
   Qed.
 
-  Global Instance term_midtape : computableTime' (@midtape sig) (fun _ _ => (1, fun _ _ => (1,fun _ _ => (1,tt)))).
+  Global Instance term_midtape : computable (@midtape sig).
   Proof.
-    extract constructor. solverec.
+    extract constructor.
   Qed.
   
 End reg_tapes.
@@ -114,60 +77,41 @@ End reg_tapes.
 
 Section fix_sig.
   Variable sig : finType.
-  Context `{reg_sig : encodable sig}.
+  Context `{reg_sig : registered sig}.
 
 
   Definition mconfigAsPair {B : finType} {n} (c:mconfig sig B n):= let (x,y) := c in (x,y).
 
-  Global Instance encodable_mconfig (B : finType) `{encodable B} n: encodable (mconfig sig B n).
+  Global Instance registered_mconfig (B : finType) `{registered B} n: registered (mconfig sig B n).
   Proof using reg_sig.
-    eapply (registerAs mconfigAsPair).
-  Defined.
+    eapply (registerAs mconfigAsPair). clear.
+    register_inj.
+  Defined. (* because registerAs *)
 
-  Global Instance term_mconfigAsPair (B : finType) `{encodable B} n: computableTime' (@mconfigAsPair B n) (fun _ _ => (1,tt)).
+  Global Instance term_mconfigAsPair (B : finType) `{registered B} n: computable (@mconfigAsPair B n).
   Proof.
-    apply cast_computableTime.
+    apply cast_computable.
   Qed.
 
-  Global Instance term_cstate (B : finType) `{encodable B} n: computableTime' (@cstate sig B n) (fun _ _ => (7,tt)).
+  Global Instance term_cstate (B : finType) `{registered B} n: computable (@cstate sig B n).
   Proof.
-    apply computableTimeExt with (x:=fun x => fst (mconfigAsPair x)).
-    2:{extract. solverec. }
+    apply computableExt with (x:=fun x => fst (mconfigAsPair x)).
+    2:{extract. }
     intros [];reflexivity.
   Qed.
 
-  Global Instance term_ctapes (B : finType) `{encodable B} n: computableTime' (@ctapes sig B n) (fun _ _ => (7,tt)).
+  Global Instance term_ctapes (B : finType) `{registered B} n: computable (@ctapes sig B n).
   Proof.
-    apply computableTimeExt with (x:=fun x => snd (mconfigAsPair x)).
-    2:{extract. solverec. }
+    apply computableExt with (x:=fun x => snd (mconfigAsPair x)).
+    2:{extract. }
     intros [];reflexivity.
   Qed.
 
-  Global Instance encodable_mk_mconfig (B : finType) `{encodable B} n: computableTime' (@mk_mconfig sig B n) (fun _ _ => (1,fun _ _ => (3,tt))).
+  Global Instance registered_mk_mconfig (B : finType) `{registered B} n: computable (@mk_mconfig sig B n).
   Proof.
     computable_casted_result.
-    extract. solverec.
+    extract.
   Qed.
 End fix_sig.
 
 #[export] Hint Resolve tape_enc_correct : Lrewrite.
-
-Import PrettyBounds.SizeBounds.
-
-Lemma sizeOfTape_by_size {sig} `{encodable sig} (t:(tape sig)) :
-  sizeOfTape t <= size (enc t).
-Proof.
-  unfold enc;cbn.
-  destruct t;cbn [tapeToList sizeOfTape length size].
-  all:rewrite ?app_length,?rev_length. all:cbn [length].
-  all:ring_simplify. all:try rewrite !size_list_enc_r. all:try nia.
-Qed.
-
-Lemma sizeOfmTapes_by_size {sig} `{encodable sig} n (t:tapes sig n) :
-  sizeOfmTapes t <= size (enc t).
-Proof.
-  setoid_rewrite enc_vector_eq. rewrite Lists.size_list.
-  erewrite <- sumn_map_le_pointwise with (f1:=fun _ => _). 2:{ intros. setoid_rewrite <- sizeOfTape_by_size. reflexivity. }
-  rewrite sizeOfmTapes_max_list_map. unfold MaxList.max_list_map. rewrite max_list_sumn.
-  etransitivity. 2:now apply Nat.le_add_r. rewrite vector_to_list_correct. apply sumn_map_le_pointwise. intros. nia.
-Qed.
