theories/L/Tactics/LTactics.v
@@ -1,4 +1,4 @@
 From MetaCoq.Template Require Export TemplateMonad.Core.
 
 (* * Certifying extraction from Coq to L with time bounds *)
-From Undecidability.L.Tactics Require Export Lsimpl mixedTactics ComputableTime Lbeta Computable ComputableTactics Lproc Lrewrite.
+From Undecidability.L.Tactics Require Export Lsimpl mixedTactics Lbeta Computable ComputableTactics Lproc Lrewrite.
