theories/L/Tactics/mixedTactics.v
@@ -1,4 +1,5 @@
 Require Import Undecidability.Shared.Libs.PSL.Base Lia Ring. 
+Require Import ZArith.
 
 Tactic Notation "destruct" "_":= 
   match goal with
@@ -22,11 +23,6 @@ Ltac trace :=
   match goal with
     |- ?G => idtac "Trace:";idtac G
   end.
-
-Require Export ZArith. 
-Ltac leq_crossout :=
-       try zify;try apply Zle_0_minus_le; ring_simplify;
-       repeat eapply Z.add_nonneg_nonneg;try now (repeat eapply Z.mul_nonneg_nonneg;easy).
 
 Tactic Notation (at level 3) "repeat'" tactic3(t) :=
   let rec loop := (once t);try loop in loop.
